examples/PluginTest.v
@@ -1,16 +1,32 @@
 From QuickChick Require Import QuickChick.
 
+QuickChickDebug Debug On.
+
 Inductive Tree :=
 | Leaf : Tree
 | Node : nat -> Tree -> Tree -> Tree.
 
 Derive Arbitrary for Tree.
 
-Inductive goodTree : nat -> Tree -> Prop :=
-| GoodLeaf : forall n, goodTree n Leaf 
-| GoodNode : forall m l r, goodTree m l -> goodTree m (Node m l r).
+Inductive recursion_test : nat -> Tree -> Prop :=
+| RecLeaf : forall n, recursion_test n Leaf 
+| RecNode : forall m l r, recursion_test m l -> recursion_test m (Node m l r).
+
+Derive ArbitrarySizedSuchThat for (fun p => let (m,tr) := p in recursion_test m tr).
+
+Inductive checker_test : nat -> Tree -> Prop :=
+| CheckerLeaf : forall n, checker_test n Leaf
+| CheckerNode : forall n t, checker_test O Leaf -> checker_test n t.
+
+Instance dec_opt l t : DecOpt (checker_test l t).
+Admitted.
+
+Derive ArbitrarySizedSuchThat for (fun p => let (m,tr) := p in checker_test m tr).
+
 
                                              (* m > n -> goodTree m l -> goodTree m r -> goodTree n (Node m l r). *)
+
+
 
 Instance test_coercion A B (P : A -> B -> Prop) `{Gen B}
          {_ : forall y, GenSuchThat _ (fun x => P x y)} :
@@ -22,10 +38,3 @@ Instance test_coercion A B (P : A -> B -> Prop) `{Gen B}
 
 Definition foo : G (option (nat * nat)) :=
   @arbitraryST _ (fun p : nat * nat => let (x,y) := p in x = y) _.
-
-QuickChickDebug Debug On.
-Derive ArbitrarySizedSuchThat for (fun p => let (m,tr) := p in goodTree m tr).
-
-
-
-
